lib_misc/SeqUtils.fst
@@ -43,20 +43,20 @@ let init_nat_len (len: nat)
   (Seq.length (init_nat len) = len)
   = ()
 
-noextract
-let init_nat_refined (len: nat) (len2: nat)
-  : Pure (Seq.lseq (k:nat{k < len2}) len)
-  (requires len <= len2)
-  (ensures fun _ -> True)
-  =
-  let s : Seq.lseq (k:nat{k < len}) len
-    = Seq.init len (fun k -> k) in
-  let f : (k:nat{k < len}) -> (k':nat{k' < len2})
-    = fun k -> k in
-  Seq.map_seq_len f s;
-  let s' : Seq.lseq (k:nat{k < len2}) len
-    = Seq.map_seq f s in
-  s'
+//noextract
+//let init_nat_refined (len: nat) (len2: nat)
+//  : Pure (Seq.lseq (k:nat{k < len2}) len)
+//  (requires len <= len2)
+//  (ensures fun _ -> True)
+//  =
+//  let s : Seq.lseq (k:nat{k < len}) len
+//    = Seq.init len (fun k -> k) in
+//  let f : (k:nat{k < len}) -> (k':nat{k' < len2})
+//    = fun k -> k in
+//  Seq.map_seq_len f s;
+//  let s' : Seq.lseq (k:nat{k < len2}) len
+//    = Seq.map_seq f s in
+//  s'
 
 noextract
 let init_u32_refined (len: nat)
@@ -72,6 +72,18 @@ let init_u32_refined (len: nat)
   let s' : Seq.lseq (k:U32.t{U32.v k < len}) len
     = Seq.map_seq f s in
   s'
+
+let init_u32_refined_index (len: nat) (i:nat{i < len})
+  : Lemma
+  (requires FStar.UInt.size len U32.n)
+  (ensures Seq.index (init_u32_refined len) i = U32.uint_to_t i)
+  =
+  let s : Seq.lseq (k:nat{k < len}) len
+    = Seq.init len (fun k -> k) in
+  let f : (k:nat{k < len}) -> (k':U32.t{U32.v k' < len})
+    = fun k -> U32.uint_to_t k in
+  Seq.map_seq_len f s;
+  Seq.map_seq_index f s i
 
 let map_seq_slice_aux (#a #b:Type)
   (f: a -> Tot b)
